i2c/i2cCircuitScript.sml
@@ -17,6 +17,8 @@ Definition i2c_reg_top_ff_def:
   i2c_reg_top_ff (fext: i2c_circuit_ext_state) (s: i2c_circuit_state) (s': i2c_circuit_state) = ^i2c_reg_top_ff_tm
 End
 
+Theorem i2c_reg_top_comb_1_trans = SIMP_RULE (pure_ss ++ ARITH_ss) [reg_req_decode_def, reg_req_accfupds, combinTheory.K_THM, dimindex_7] i2c_reg_top_comb_1_def;
+
 val init_tm = add_x_inits ``
   <|
     regs := ^i2c_regs_init_tm;
