i2c/i2cRegsCircuitProofScript.sml
@@ -1,7 +1,7 @@
 open HolKernel Parse boolLib bossLib;
 open translatorLib;
 open cheshireCircuitTheory i2cCircuitStateTheory;
-open i2cRegsCircuitLib;
+open i2cRegsCircuitLib i2cMappingsTheory;
 
 val _ = new_theory "i2cRegsCircuitProof";
 
@@ -32,23 +32,241 @@ Definition i2c_circuit_def:
   i2c_circuit = mk_module (procs [i2c_reg_top_ff]) (procs [i2c_reg_top_comb_1; i2c_reg_top_comb_2]) i2c_circuit_init
 End
 
-Theorem i2c_reg_top_correct:
+Theorem procs_append:
+  ∀ps qs fext s s'. procs (ps ++ qs) fext s s' = procs qs fext s (procs ps fext s s')
+Proof
+  Induct_on `ps`
+  >> simp [procs_def]
+QED
+
+Theorem procs_unchanged:
+  !f ps fext s s'.
+  (!p fext s s'. MEM p ps ⇒ f (p fext s s') = f s') ==>
+  f (procs ps fext s s') = f s'
+Proof
+  Induct_on `ps`
+  >> simp [procs_def]
+QED
+
+Theorem COND_ARG1:
+  (if c then f g x else f h x) = f (if c then g else h) x
+Proof
+  simp [COND_RAND, COND_RATOR]
+QED
+
+Theorem COND_ARG1_K:
+  (if c then f (K a) x else f (K b) x) = f (K (if c then a else b)) x
+Proof
+  simp [COND_ARG1, GSYM COND_RAND, GSYM COND_RATOR]
+QED
+
+Theorem i2c_reg_top_comb_1_flat = i2c_reg_top_comb_1_def
+  |> SRULE [COND_ARG1_K, COND_ARG1]
+  |> SRULE [Ntimes LET_THM 5]
+  |> SRULE [SRULE [] (GSYM i2c_req_error_alt), SF boolSimps.LET_ss];
+
+Theorem i2c_reg_top_comb_2_flat = SRULE [COND_ARG1_K, COND_ARG1] i2c_reg_top_comb_2_def;
+
+Theorem i2c_reg_top_ff_flat = i2c_reg_top_ff_def
+  |> SRULE [COND_ARG1_K]
+  |> SRULE [SF boolSimps.LET_ss];
+
+Theorem word_bits_bit_field_insert:
+  h < dimindex (:'a) ∧ dimindex (:'b) = h + 1 - l ⇒
+  (h -- l) (bit_field_insert h l (v: 'b word) (w: 'a word)) = w2w v
+Proof
+  rpt strip_tac
+  >> asm_simp_tac (boss_ss () ++ fcpLib.FCP_ss) [word_bits_def, bit_field_insert_def, word_modify_def, Cong AND_CONG, w2w]
+  >> rpt strip_tac
+  >> ‘i < h + 1 − l ⇔ i + l < h + 1’ by (fs [] >> simp [DIMINDEX_GT_0])
+  >> simp [arithmeticTheory.LE_LT1]
+QED
+
+Theorem word_extract_bit_field_insert:
+  h < dimindex (:'a) ∧ dimindex (:'b) = h + 1 - l ⇒
+  (h >< l) (bit_field_insert h l (v: 'b word) (w: 'a word)) = v
+Proof
+  simp [word_extract_def, word_bits_bit_field_insert, w2w_w2w, WORD_ALL_BITS]
+QED
+
+Theorem eq_w2n_iff_eq_n2w:
+  !(w: 'a word) n. n < dimword (:'a) ==> (n = w2n w <=> w = n2w n)
+Proof
+  rpt strip_tac
+  >> iff_tac
+  >> simp []
+QED
+
+Theorem w2n_eq_iff_eq_n2w:
+  !(w: 'a word) n. n < dimword (:'a) ==> (w2n w = n <=> w = n2w n)
+Proof
+  rpt strip_tac
+  >> iff_tac
+  >- (strip_tac
+      >> first_x_assum (assume_tac o GSYM)
+      >> simp [eq_w2n_iff_eq_n2w])
+  >- simp []
+QED
+
+Theorem i2c_reg_top_comb_2_i2c_read:
+  st.regs = s.regs ∧ i2c_hwext_read_rel st s'.hw2reg ⇒
+  (33 >< 2) (i2c_reg_top_comb_2 fext s s').reg_rsp_o =
+  case i2c_read st nb (w2n s'.addr) of
+    INL _ => 0xFFFFFFFFw
+  | INR (_, value) => value
+Proof
+  simp [i2c_hwext_read_rel_def, i2c_reg_top_comb_2_flat, word_extract_bit_field_insert]
+  >> rpt IF_CASES_TAC
+  >> simp [i2c_read_def, w2n_eq_iff_eq_n2w]
+QED
+
+Theorem mk_circuit_cstep:
+  ∀sstep cstep s fext n. ∃s'. mk_circuit sstep cstep s fext n = cstep (fext n) s' s'
+Proof
+  rpt strip_tac
+  >> Cases_on ‘n’
+  >- (qexists ‘s’ >> simp [mk_circuit_def])
+  >- (qexists ‘(sstep (fext n') (mk_circuit sstep cstep s fext n')
+                      (mk_circuit sstep cstep s fext n'))’
+      >> simp [mk_circuit_def])
+QED
+
+Theorem word_bit_bit_field_insert:
+  i < l \/ h < i ==> word_bit i (bit_field_insert h l a b) = word_bit i b
+Proof
+  asm_simp_tac (boss_ss () ++ fcpLib.FCP_ss) [word_bit_def, bit_field_insert_def, word_modify_def, arithmeticTheory.SUB_LESS_OR_EQ, Cong AND_CONG]
+QED
+
+(* For some reason `simp` vehemently refuses to use the original `FCP_APPLY_UPDATE_THM`. *)
+Theorem FCP_APPLY_UPDATE_THM_2:
+  !(m: 'a['b]) a w b. b < dimindex (:'b) ==> (a :+ w) m ' b = if a = b then w else m ' b
+Proof
+  assume_tac fcpTheory.FCP_APPLY_UPDATE_THM >> simp []
+QED
+
+Theorem ISL_SUM_MAP:
+  !f g z. ISL (SUM_MAP f g z) = ISL z
+Proof
+  Cases_on `z` >> simp []
+QED
+
+Theorem nb_wstrb:
+  !(wstrb: word4) nb n.
+  (!i. word_bit i wstrb <=> i < nb) /\ n + 1 = dimindex (:'b) ==>
+  (nb > n <=> ((n >< 0) wstrb: 'b word) = -1w)
+Proof
+  rpt strip_tac
+  >> full_simp_tac (boss_ss () ++ fcpLib.FCP_ss) [arithmeticTheory.GREATER_DEF, word_bit_def, word_extract_def, WORD_NEG_1_T, w2w, word_bits_def, Cong AND_CONG, arithmeticTheory.LE_LT1]
+  >> iff_tac
+  >> simp []
+QED
+
+val all_ones_rewrites = map (fn n => ``-1w: ^(n |> Arbnum.fromInt |> fcpLib.index_type |> ty_antiq) word`` |> EVAL |> GSYM |> Once) [1, 2, 3, 4];
+
+Theorem i2c_req_error_i2c_write:
+  !(req: 7 reg_req) st nb.
+  req.valid /\ req.write /\ (∀i. word_bit i req.wstrb ⇔ i < nb) ==>
+  i2c_req_error req = ISL (i2c_write st nb (w2n req.addr) req.wdata)
+Proof
+  rpt strip_tac
+  >> asm_simp_tac std_ss [i2c_write_def, dimword_def, dimindex_7, w2n_eq_iff_eq_n2w]
+  >> rpt TOP_CASE_TAC
+  >> (simp [i2c_req_error_def]
+      (* We need to re-evaluate this every time so that Once doesn't mark itself as
+       * used after the first subgoal and fail to apply these to any of the others. *)
+      >> goal_term (fn _ => pure_rewrite_tac (map Once all_ones_rewrites))
+      >> dep_rewrite.DEP_REWRITE_TAC [GSYM nb_wstrb]
+      >> simp [])
+QED
+
+Theorem i2c_req_error_i2c_read:
+  !(req: 7 reg_req) st nb.
+  req.valid /\ ~req.write ==>
+  i2c_req_error req = ISL (i2c_read st nb (w2n req.addr))
+Proof
+  rpt strip_tac
+  >> simp [i2c_read_def, w2n_eq_iff_eq_n2w]
+  >> rpt IF_CASES_TAC
+  >> simp [i2c_req_error_def]
+QED
+
+Theorem i2c_reg_top_rsp_correct:
   let
     i2c = mk_module (procs (ffs1 ++ [i2c_reg_top_ff] ++ ffs2)) (procs ([i2c_reg_top_comb_1] ++ combs ++ [i2c_reg_top_comb_2])) i2c_circuit_init;
     req = reg_req_decode (fext n).reg_req_i: 7 reg_req;
     oracle_res = if ~req.valid then
       INR (I, NONE, NONE)
     else if req.write then
-      SUM_MAP (\(st_upd, notif). (st_upd, notif, NONE)) I (i2c_write st nb (w2n req.addr) req.wdata)
+      SUM_MAP I (\(st_upd, notif). (st_upd, notif, NONE)) (i2c_write st nb (w2n req.addr) req.wdata)
     else
-      SUM_MAP (\(notif, rdata). (I, notif, rdata)) I (i2c_read st nb (w2n req.addr));
-    rsp = reg_rsp_decode (i2c fext fbits (SUC n)).reg_rsp_o;
+      SUM_MAP I (\(notif, rdata). (I, notif, SOME rdata)) (i2c_read st nb (w2n req.addr));
+    rsp = reg_rsp_decode (i2c fext fbits n).reg_rsp_o;
   in
-  (!proc fext s s'. proc IN set (ffs1 ++ ffs2 ++ combs) ==>
+  (!proc fext s s'. MEM proc combs ==>
     let
       s'' = proc fext s s'
     in
-      s''.reg2hw = s'.reg2hw /\ s''.reg_rsp_o = s'.reg_rsp_o)
+      s''.regs = s'.regs /\ s''.reg_rsp_o = s'.reg_rsp_o
+      /\ s''.addr = s'.addr /\ s''.write = s'.write /\ s''.wdata = s'.wdata
+      /\ s''.wstrb = s'.wstrb /\ s''.valid = s'.valid)
+  /\ i2c_state_rel st (i2c fext fbits n)
+  /\ (!i. word_bit i req.wstrb <=> i < nb)
+  ==> rsp.ready
+    /\ rsp.error = ISL oracle_res
+    /\ (!st_upd notif rdata. oracle_res = INR (st_upd, notif, SOME rdata) ==> rsp.rdata = rdata)
+Proof
+  qpat_abbrev_tac `sstep = procs (_ ++ ffs2)`
+  >> qpat_abbrev_tac `cstep = procs (_ ++ [i2c_reg_top_comb_2])`
+  >> simp []
+  >> rpt strip_tac
+  >> `?s'. mk_circuit sstep cstep (i2c_circuit_init fbits) fext n = cstep (fext n) s' s'` by irule mk_circuit_cstep
+  >> unabbrev_all_tac
+  >> fs [mk_module_def, procs_def, procs_append, reg_rsp_decode_def]
+  (* ready *)
+  >- (simp [i2c_reg_top_comb_2_flat, word_bit_bit_field_insert]
+      >> simp [procs_unchanged, i2c_reg_top_comb_1_flat, word_bit_def, FCP_APPLY_UPDATE_THM_2])
+  (* error *)
+  >- (simp [i2c_reg_top_comb_2_flat, word_bit_bit_field_insert]
+      >> simp [procs_unchanged, i2c_reg_top_comb_1_flat, word_bit_def, FCP_APPLY_UPDATE_THM_2]
+      >> rpt IF_CASES_TAC
+      >- simp [i2c_req_error_def]
+      >- fs [ISL_SUM_MAP, i2c_req_error_i2c_write]
+      >- fs [ISL_SUM_MAP, i2c_req_error_i2c_read])
+  (* rdata *)
+  >- (dep_rewrite.DEP_REWRITE_TAC [i2c_reg_top_comb_2_i2c_read]
+      >> `!fext s s'. (i2c_reg_top_comb_1 fext s s').regs = s'.regs` by simp [i2c_reg_top_comb_1_flat]
+      >> `!fext s s'. (i2c_reg_top_comb_2 fext s s').regs = s'.regs` by simp [i2c_reg_top_comb_2_flat]
+      >> `st.regs = (i2c_reg_top_comb_2 (fext n) s' (procs combs (fext n) s' (i2c_reg_top_comb_1 (fext n) s' s'))).regs` by fs [i2c_state_rel_def, i2c_core_state_rel_def]
+      >> rfs [procs_unchanged]
+      >> `!fext s s'. (i2c_reg_top_comb_2 fext s s').hw2reg = s'.hw2reg` by simp [i2c_reg_top_comb_2_flat]
+      >> `i2c_hwext_read_rel st (i2c_reg_top_comb_2 (fext n) s' (procs combs (fext n) s' (i2c_reg_top_comb_1 (fext n) s' s'))).hw2reg` by fs [i2c_state_rel_def, i2c_core_state_rel_def]
+      >> rfs []
+      >> `(reg_req_decode (fext n).reg_req_i: 7 reg_req).valid` by (spose_not_then assume_tac >> fs [])
+      >> `~(reg_req_decode (fext n).reg_req_i: 7 reg_req).write`
+         by (spose_not_then assume_tac
+             >> Cases_on `i2c_write st nb (w2n (reg_req_decode (fext n).reg_req_i: 7 reg_req).addr) (reg_req_decode (fext n).reg_req_i: 7 reg_req).wdata`
+             >> fs [sumTheory.SUM_MAP_def]
+             >> Cases_on `y`
+             >> fs [])
+      >> Cases_on `i2c_read st nb (w2n (reg_req_decode (fext n).reg_req_i: 7 reg_req).addr)`
+      >- fs []
+      >- (Cases_on `y`
+          >> fs []
+          >> simp [i2c_reg_top_comb_1_flat]))
+QED
+
+Theorem i2c_reg_top_i2c_state_rel_step:
+  let
+    i2c = mk_module (procs (ffs1 ++ [i2c_reg_top_ff] ++ ffs2)) (procs ([i2c_reg_top_comb_1] ++ combs ++ [i2c_reg_top_comb_2])) i2c_circuit_init;
+    req = reg_req_decode (fext n).reg_req_i: 7 reg_req;
+    oracle_res = if ~req.valid then
+      INR (I, NONE, NONE)
+    else if req.write then
+      SUM_MAP I (\(st_upd, notif). (st_upd, notif, NONE)) (i2c_write st nb (w2n req.addr) req.wdata)
+    else
+      SUM_MAP I (\(notif, rdata). (I, notif, SOME rdata)) (i2c_read st nb (w2n req.addr));
+  in
+  (!proc fext s s'. MEM proc (ffs1 ++ ffs2 ++ combs) ==> (proc fext s s').reg2hw = s'.reg2hw)
   /\ (!st fext fbits n notif. i2c_state_rel st (i2c fext fbits n)
     (* TODO: the other way to do this would be to compare notif to
      * (i2c_reg_top_comb_1 (fext n) (i2c fext fbits n) (i2c fext fbits n)).reg2hw;
@@ -60,12 +278,10 @@ Theorem i2c_reg_top_correct:
     ==> ?fnums. i2c_core_state_rel (i2c_tick notif (st with fnums := fnums)) (i2c fext fbits (SUC n)))
   /\ i2c_state_rel st (i2c fext fbits n)
   /\ (!i. word_bit i req.wstrb <=> i < nb)
-  ==> rsp.ready
-    /\ rsp.error = ISR oracle_res
-    /\ (?st_upd notif rdata. oracle_res = INR (st_upd, notif, rdata)
-      ==> (?fnums. i2c_state_rel (st_upd (i2c_tick notif (st with fnums := fnums))) (i2c fext fbits (SUC n)))
-        /\ (!value. rdata = SOME value ==> rsp.rdata = value))
+  /\ oracle_res = INR (st_upd, notif, rdata)
+  ==> ?fnums. i2c_state_rel (st_upd (i2c_tick notif (st with fnums := fnums))) (i2c fext fbits (SUC n))
 Proof
+  cheat
 QED
 
 val _ = export_theory ();
